tests/CountBy/CountBy.v
@@ -54,6 +54,16 @@ Section WithCava.
   Definition countBy : signal (Vec Bit 8) -> cava (signal (Vec Bit 8))
     := loopDelayS addN.
 
+  (* A version that uses loopDelaySRAlt *)
+  Definition countByAlt : signal (Vec Bit 8) -> cava (signal (Vec Bit 8))
+    := loopDelaySRAlt (tupleInterfaceDefault [Vec Bit 8]) addN.
+
+  (* A use of loopDelaySRAlt that has a composite signal which in this case
+     is a toggling output bit in the second element of the state pair. *)
+  Definition countByInvAlt : signal (Vec Bit 8) -> cava (signal (Vec Bit 8) * signal Bit)
+    := loopDelaySRAlt (tupleInterfaceDefault [Vec Bit 8; Bit])
+       (pairLeft >=> first addN >=> second inv).
+
 End WithCava.
 
 (* Convenience notations for certain bytes *)
@@ -69,6 +79,15 @@ Definition b250 := N2Bv_sized 8 250.
 Local Open Scope list_scope.
 
 Example countBy_ex1: sequential (countBy [b14; b7; b3; b250]) = [b14; b21; b24; b18].
+Proof. reflexivity. Qed.
+
+(* Check loopDelaySRAlt version *)
+Example countByAlt_ex1: sequential (countByAlt [b14; b7; b3; b250]) = [b14; b21; b24; b18].
+Proof. reflexivity. Qed.
+
+(* Check the toggling output version. *)
+Example countByInvAlt_ex1: sequential (countByInvAlt [b14; b7; b3; b250])
+  = ([b14; b21; b24; b18], [true; false; true; false]).
 Proof. reflexivity. Qed.
 
 Definition countBy_Interface
@@ -88,3 +107,37 @@ Definition countBy_tb_expected_inputs := sequential (countBy countBy_tb_inputs).
 Definition countBy_tb
   := testBench "countBy_tb" countBy_Interface
      countBy_tb_inputs countBy_tb_expected_inputs.
+
+(* Also generate netlist for loopDelaySRAlt version *)
+
+Definition countByAlt_Interface
+  := sequentialInterface "countByAlt"
+     "clk" PositiveEdge "rst" PositiveEdge
+     [mkPort "i" (Vec Bit 8)]
+     [mkPort "o" (Vec Bit 8)]
+     [].
+
+Definition countByAlt_Netlist := makeNetlist countByAlt_Interface countByAlt.
+
+Definition countByAlt_tb
+  := testBench "countByAlt_tb" countBy_Interface
+     countBy_tb_inputs countBy_tb_expected_inputs.
+
+(* Check netlist generation for loops with composite feedback. *)
+
+Definition countByInvAlt_Interface
+  := sequentialInterface "countByInvAlt"
+     "clk" PositiveEdge "rst" PositiveEdge
+     [mkPort "i" (Vec Bit 8)]
+     [mkPort "o" (Vec Bit 8); mkPort "t" Bit]
+     [].
+
+Definition countByInvAlt_Netlist := makeNetlist countByInvAlt_Interface countByInvAlt.
+
+Definition countByInvAlt_tb
+  := testBench "countByInvAlt_tb" countByInvAlt_Interface
+     countBy_tb_inputs [(b0, false); (b14, true); (b21, false); (b24, true); (b18, false)].
+
+(* Question: why does the Example testbench above not produce the output for the first
+   cycle i.e. (b0, false) ? 
+*)
